\documentclass[fleqn,12pt]{article}
\usepackage[top=2cm, left=2cm,right=3cm,bottom=2cm]{geometry}
%\usepackage[fleqn]{amsmath}
\usepackage{amsmath}
\usepackage{url,enumerate}
\usepackage{color,hyperref,enumerate,multicol}
\usepackage{cleveref}
\usepackage{ifthen}
\newboolean{answers}
%\setboolean{answers}{true}  % set to true to include TODO statements
\setboolean{answers}{false}  % set to false to use input statements
\usepackage{amssymb}
\usepackage{tikz}
\newcommand{\<}{\ensuremath{\langle}}
\renewcommand{\>}{\ensuremath{\rangle}}
\newcommand{\Z}{\ensuremath{\mathbb{Z}}}
\newcommand{\N}{\ensuremath{\mathbb{N}}}
\newcommand{\ur}{\ensuremath{\underline{\mathrm{r}}}}
\newcommand{\uT}{\ensuremath{\underline{\mathrm{T}}}}
\newcommand{\uF}{\ensuremath{\underline{\mathrm{F}}}}
\newcommand{\uN}{\ensuremath{\underline{\mathrm{N}}}}
\newcommand{\ui}{\ensuremath{\underline{\mathrm{i}}}}
\newcommand{\uj}{\ensuremath{\underline{\mathrm{j}}}}
\newcommand{\ua}{\ensuremath{\underline{\mathrm{a}}}}
\newcommand{\ub}{\ensuremath{\underline{\mathrm{b}}}}
\newcommand{\un}{\ensuremath{\underline{\mathrm{n}}}}
\newcommand{\uv}{\ensuremath{\underline{\mathrm{v}}}}
\newcommand{\Sym}{\ensuremath{\operatorname{Sym}}}
\newcommand{\id}{\ensuremath{\operatorname{id}}}
\newcommand{\bG}{\ensuremath{\mathbf{G}}}
\newcommand{\ba}{\ensuremath{\mathbf{a}}}
\newcommand{\bv}{\ensuremath{\mathbf{v}}}
\newcommand{\bb}{\ensuremath{\mathbf{b}}}
\newcommand{\bA}{\ensuremath{\mathbf{A}}}
\newcommand{\bB}{\ensuremath{\mathbf{B}}}
\newcommand{\bS}{\ensuremath{\mathbf{S}}}
\newcommand{\bT}{\ensuremath{\mathbf{T}}}
\newcommand{\bc}{\ensuremath{\mathbf{c}}}
\newcommand{\bi}{\ensuremath{\mathbf{i}}}
\newcommand{\bj}{\ensuremath{\mathbf{j}}}
\newcommand{\meet}{\ensuremath{\wedge}}
\newcommand{\join}{\ensuremath{\vee}}
\newcommand{\dotsize}{1pt}
\crefformat{footnote}{#2\footnotemark[#1]#3}

\begin{document}
%\thispagestyle{empty}
\pagestyle{empty}
%\fontsize{11.5}{13.8}
% \fontsize{14}{17}
% \selectfont
\noindent {\bf MATH 301 - Section B}
\hfill {\bf Fall 2014}
\begin{center}
{\bf Midterm Exam 2 -- SOLUTIONS}
\thispagestyle{empty}
%% covers sections 5.1--5.5 and 7.1--7.4
\end{center}

\bigskip

\begin{enumerate}[{\bf 1.}]
\item Give precise definitions of the following:

  \begin{enumerate}
  %% \item {\bf algebra}
  %%   \vskip4cm
  \item {\bf $n$-ary operation} on a set $A$

    \medskip

    An {\bf $n$-ary operation} on a set $A$ is a function,
    $f: A^n \rightarrow A$, with domain $A^n$ and codomain $A$.

    \bigskip

  \item {\bf $n$-ary relation} on a set $A$

    \medskip

    An {\bf $n$-ary relation} on a set $A$ is a subset of $A^n$.

    \bigskip

  \item {\bf algebra} or {\bf algebraic structure}

    \medskip

    An {\bf algebra} or {\bf algebraic structure} is a pair $\<A, F\>$ consisting of a
    nonempty set $A$ along with a set $F$ of operations on $A$.

    \bigskip

  \item {\bf relational structure}

    \medskip

    An {\bf relational structure} is a pair $\<A, R\>$ consisting of a
    nonempty set $A$ along with a set $R$ of relations on $A$.

    \bigskip

  \item {\bf group homomorphism}

    \medskip

    A {\bf group homomorphism} is a function 
    $\varphi: G \rightarrow H$ from a group $G$ to a group $H$ satisfying,
    for all $x, y \in G$, $\varphi(x\cdot y) = \varphi(x) \cdot \varphi(y)$.

    \bigskip

  \item {\bf normal subgroup}
    \medskip

    A {\bf normal subgroup} of a group $G$ is a subgroup $N\leq G$ such that
    any one (hence all) of the following equivalent conditions holds for all $g\in G$:
    \begin{enumerate}
    \item $g N g^{-1} = N$;
    \item $g N = Ng$;
    \item $g n g^{-1} \in N$, for all $n\in N$.
    \end{enumerate}

    \bigskip


  \end{enumerate}

\newpage

\item
  \begin{enumerate}
  \item State \emph{Lagrange's Theorem} about the order of a group and its
    subgroups. (Be sure to state all assumptions that are needed in order for
    the theorem to hold.)  

    \medskip

    {\bf Theorem.} Let $G$ be a finite group and let $H$ be a subgroup
    of $G$. Then $|G|/|H| = [G : H]$ is the number of distinct left cosets of $H$ in
    $G$. In particular, the number of elements in $H$ must divide the number of
    elements in $G$.

    \bigskip

    \item Recall that $G$ is the \emph{internal direct product} of the subgroups
      $H$ and $K$ if $G = HK$, and $H\cap K= \{e\}$, and $H$ and $K$ centralize
      each other (i.e., $hk = kh$ for all $h\in H$ and $k\in
      K$).\footnote{\label{note1}Note to students: On the actual exam, I left
        out the condition that $G = HK$. (Points were not deducted from
        answers that didn't check this condition.)}

\medskip

      Suppose $G$ has order 28 and subgroups $H$ and $K$ of orders 4
      and 7 respectively which centralize each other.  Prove that
      $G$ is the internal direct product of $H$ and $K$.

      \medskip

      \noindent {\bf Solution:} 
      Since we are already given that $hk = kh$ for all $h\in H$ and $k\in K$, we 
      must show that $H\cap K= \{e\}$ and $G = HK$.\cref{note1}

      \medskip
      Suppose $x \in H\cap K$, then $x \in H$ implies $\<x\>$ is a subgroup of $H$ so,
      by Lagrange's Theorem $|x|$ divides $|H| = 4$.
      Similarly $x \in K$ implies $\<x\>$ is a subgroup of $K$ so,
      by Lagrange's Theorem $|x|$ divides $|K| = 7$. Since $|x|$ divides both 4 and 7,
      we must have $|x| = 1$, so $x = e$.  That is $H\cap K = \{e\}$.

      \medskip
      Finally, we show that $G = HK$.\cref{note1}
      Since $[G : K] = |G|/|K| = 28/7 = 4$, there are four cosets of
      $K$ in $G$ and, since $H\cap K = \{e\}$, we can list these four cosets
      using as representatives the four distinct elements of $H$. That is,
      the cosets of $K$ in $G$ are $K, h_1K, h_2K, h_3K$.  Since any group is
      the disjoint union of the cosets of any of its subgroups, we have
      $G = K \cup h_1K \cup h_2K \cup h_3K = HK$.
  \end{enumerate}
\newpage
\item {\bf Prove either (a) OR (b) OR (c).} If you prove more than one, circle
  the letter of the one you want graded.

\begin{enumerate}
\item
If $G \cong H$ and $G$ is cyclic, then $H$ is cyclic.

\item If a group $G$ has a subgroup $H$ of index 2, then $H$ is
normal in $G$. \\
Conclude that $A_n \triangleleft S_n$ for $n \geq 3$.

\item 
If a group $G$ has exactly one subgroup $H$ of order $k$, then
$H$ is normal in $G$. 

\end{enumerate}

\medskip
\noindent {\bf Solution:}
\begin{enumerate}
\item
{\bf Claim:} If $G \cong H$ and $G$ is cyclic, then $H$ is cyclic.

\medskip

{\bf Proof:}
 Suppose $G = \<a\> \cong H$ and suppose 
$\varphi: G \rightarrow H$ is an isomorphism.  Then 
$H = \<\varphi(a)\>$.  To see this, fix $h\in H$.  We will show 
$h = (\varphi(a))^k$ for some $k\in \N$. Indeed, let $b = \varphi^{-1}(h)$.
Since $b\in G = \<a\>$, we must have $b = a^k$ for some $k\in \N$.
Also, $\varphi(a^k) = (\varphi(a))^k$, since $\varphi$ is a homomorphism. 
Therefore, $(\varphi(a))^k = \varphi(a^k) = \varphi(b) = \varphi(\varphi^{-1}(h)) = h$.



\bigskip

\item {\bf Claim:} If a group $G$ has a subgroup $H$ of index 2, then $H$ is
normal in $G$. \\
Conclude that $A_n \triangleleft S_n$ for $n \geq 3$.

\medskip

{\bf Proof:}
If $[G:H]=2$, then there are two left cosets of $H$ in $G$.
Pick a $g \in G$ with $g \notin H$. 
Then the two left cosets of $H$ in $G$, 
are $H$ and $gH$. Recall that the set of left cosets partitions the group into
a \emph{disjoint} union. In the present case, $G = H \cup gH$.  
Similarly, the two right cosets of $H$ in
$G$ must be $H$ and $Hg$, and again we have a partition of $G$ as
the \emph{disjoint} union of sets $G = H \cup Hg$.  It follows that $gH = G-H = Hg$.

\medskip
Finally, since $[S_n : A_n] = 2$ for $n\geq 3$, we have $A_n \triangleleft S_n$.

\bigskip

\item 
{\bf Claim:}
If a group $G$ has exactly one subgroup $H$ of order $k$, then
$H$ is normal in $G$. 

\medskip

{\bf Proof:}
Given a subgroup $H\leq G$, and an arbitrary element $g\in G$, 
the set $gHg^{-1} := \{ghg^{-1} | h\in H\}$ is also a subgroup of $G$.
Moreover, the function $h \mapsto ghg^{-1}$ is a bijection.
Therefore, $|H| = |gHg^{-1}|$.  If $|H| =k$ and if $H$ is the only
subgroup of order $k$, then, since $|gHg^{-1}| = k$, we must have 
$H = gHg^{-1}$.
Since $g$ was arbitrary, this proves that $H$ is normal in $G$.

\end{enumerate}


\newpage

\item The {\bf center} of a group $G$ is
$Z(G) = \{ x \in G : xg = gx \text{ for all $g \in G$ }\}$.
%% We proved that $Z(G) \triangleleft G$, so the set $G / Z(G)$ of cosets forms a
%% group. Also, we proved that $G$ is abelian if $G/Z(G)$ is cyclic.

\begin{enumerate}
 \item
Show that the center of any group is a normal subgroup.

\medskip

\noindent
{\bf Solution:} Fix arbitrary $z \in Z(G)$ and $a \in G$.
Since $z$ belongs to  $Z(G)$, it commutes with every element of $G$.
Therefore, $aza^{-1} = aa^{-1}z = e z  = z\in Z(G)$, so 
$Z(G) \triangleleft G$.

\bigskip

\item
The dihedral group $D_4$ (symmetries of the square) can be
described as the permutation group with two generators 
$\rho = (1234)$ and $\mu = (13)$ satisfying $\rho^4= e = \mu^2$.
Therefore, the elements of $D_4$ are 
$\{e, \rho, \rho^2, \rho^3, \mu, \rho \mu, \rho^2 \mu, \rho^3 \mu\}$.

Calculate $Z(D_4)$, the center of $D_4$. [Hint: only one nonidentity
element of $D_4$ commutes with all other elements of $D_4$, and finding
this element should not require too much calculation.]
 

\medskip

\noindent
{\bf Solution:} 
For easy reference we make a table displaying the elements of the group.
\begin{center}
\begin{tabular}{c|c|c|c|c|c|c|c}
$e$ & $ \rho$ & $ \rho^2$ & $ \rho^3$ & $ \mu$ & $ \rho \mu$ & $ \rho^2 \mu$ & $ \rho^3 \mu$\\
\hline
$(~)$ & $ (1234)$ & $ (13)(24)$ & $ (1432)$ & $ (13)$ & $ (14)(23)$ & $ (24)$ & $(12)(34)$
\end{tabular}

\end{center}
Note that $\rho^2 = (13)(24) = (24)(13)$, and $\rho^2$ 
commutes with both generators. Indeed,
\[\rho^2 \rho = \rho^3 = \rho \rho^2 \qquad \text{ and  } \qquad
\rho^2 \mu = (13)(24)(13) = (13)(13)(24) = \mu \rho^2.
\]
Therefore, $\rho^2$ commutes with every element of $D_4$, 
so $\rho^2 \in Z(D_4)$.

From the following calculations, we see that none of the other nonidentity
elements of $D_4$ belongs to the center:
\begin{align*}
\mu \rho &= (13)(1234) = (12)(34) \\
\rho \mu &= (1234)(13) = (14)(23) \quad \Rightarrow \quad \mu \rho \neq \rho \mu,
\end{align*}
so $\mu \notin Z(D_4)$ and $\rho \notin Z(D_4)$.
\begin{align*}
\rho^3 \mu &= (1432)(13) = (12)(34)\\
\mu \rho^3&= (13)(1432) = (14)(23) \quad \Rightarrow \quad \mu \rho^3 \neq \rho^3 \mu,
\end{align*}
so $\rho^3 \notin Z(D_4)$. From this and the fact that $\rho^2$ commutes with
everything, we also have
$\rho^2 \mu \rho = \mu \rho^2 \rho = \mu \rho^3 \neq \rho^3 \mu = \rho\rho^2 \mu$, so $\rho^2\mu \notin Z(D_4)$.
%% \begin{align*}
%% \rho^2 \mu \cdot \rho &= (24)(1234) = (14)(23)\\
%% \rho \cdot \rho^2 \mu &= (1234)(24) = (12)(34)
%%  \quad \Rightarrow \quad 
%% \rho^2 \mu \cdot \rho \neq
%% \rho \cdot \rho^2 \mu, 
%% \end{align*}
\begin{align*}
\rho^3 \cdot \rho\mu &= \mu =(13) \qquad \text{ (since $\rho^4 = (~)$)}\\
\rho \mu \cdot \rho^3 &= (1234)(13)(1432) = (24) \quad \Rightarrow \quad 
\rho^3 \cdot \rho \mu \neq \rho \mu \cdot \rho^3,
\end{align*}
so %% $\rho^3 \notin Z(D_4)$ and 
$\rho \mu \notin Z(D_4)$.  Finally,
\begin{align*}
\rho^3 \mu \cdot \mu &= \rho^3 = (1432)\\
\mu \cdot \rho^3 \mu &= (13)(12)(34) = (1234)
%% \rho \mu \cdot \rho^3 &= (1234)(13)(1432) = (24) \quad \Rightarrow \quad 
%% \rho^3 \cdot \rho \mu \neq \rho \mu \cdot \rho^3,
\end{align*}
so $\rho^3 \mu \notin Z(D_4)$.
%% \begin{align*}
%% \rho^2 \mu \cdot \rho &= (24)(1234) = (14)(23)\\
%% \rho \cdot \rho^2 \mu &= (1234)(24) = (12)(34)
%%  \quad \Rightarrow \quad 
%% \rho^2 \mu \cdot \rho \neq
%% \rho \cdot \rho^2 \mu, 
%% \end{align*}
%% so $\rho^2 \mu \notin Z(D_4)$.

\medskip

 
 \item
Is $D_4/Z(D_4)$ cyclic?  Explain. [Hint: Recall, $G$ is abelian if $G/Z(G)$ is cyclic.]

\medskip

Since $D_4$ is nonabelian, $D_4/Z(D_4)$ is not cyclic.
\end{enumerate}
\newpage
\item State the First Isomorphism Theorem and use it to prove that every group
  $G$ is isomorphic to a subgroup of $\Sym(G)$. [Hint: show that a certain
  function $\lambda : G \rightarrow \Sym(G)$ is a homomorphism with trivial
  kernel.]

\medskip

  {\bf First Isomorphism Theorem.}

  Suppose $\varphi: G \rightarrow H$ is a group homomorphism
  and 
  \[
  N := \varphi^{-1}(\{e_H\}) = \{g\in G: \varphi(g) = e_H\}.
  \]
  Then there is a group isomorphism $\psi : G/N \rightarrow \varphi(G)$ such
  that $\psi \pi = \varphi$. 

  %% (The conclusion says that, for all $g\in G$, 
  %% $\psi \pi(g) = \varphi(g)$ or $\psi(gN) = \varphi(g)$.)

Let $\bG = \<G, \cdot, ^{-1}, e\>$ be a finite group of order $n$.  
Take the set $G$ (the elements of $\bG$) and consider the group of all
permutations of these elements.  We will denote this group by
$\Sym(G) = \<S, \circ, ^{-1}, \id\>$.
Fix an element $a\in G$ and recall that the function
$\lambda_a: G \rightarrow G$, defined by $\lambda_a(g) = a\cdot g$, is a
permutation of the set $G$.  That is, $\lambda_a$ belongs to the
permutation group $\Sym(G)$.  
The function $\lambda: G \rightarrow \Sym(G)$ defined by 
$a\mapsto \lambda_a$ is a group homomorphism.\footnote{Note that the function
is given, for each $a\in G$, by $\lambda(a) = \lambda_a$.}
To see this, fix $a, b \in G$.  We must show that
the permutation 
$\lambda(a\cdot b) = \lambda_{ab}$
is the same as the permutation 
$\lambda(a) \circ \lambda(b) = \lambda_a \circ \lambda_b$.
Indeed, for all $g \in G$,
\begin{align*}
\lambda_{ab} (g) &= (a\cdot b) \cdot g = a \cdot (b \cdot g) \qquad (\text{associativity})\\
&= a \cdot \lambda_b(g) = \lambda_a (\lambda_b(g)) \\
& = (\lambda_a \circ \lambda_b)(g).
\end{align*}

Therefore, by the First Isomorphism Theorem, there is a group homomorphism 
$\psi : G/N \rightarrow \Sym(G)$ such that $\psi \pi = \varphi$. Here,
$N := \lambda^{-1}(\{\id\}) = \{a\in G: \lambda_a = \id\}$ where
$\id$ is the identity permutation in $\Sym(G)$, that is $\id(g) =g$.  Also note
that, since $\psi$ is a group homomorphism, the image of $G/N$ under $\psi$ is a
subgroup of $\Sym(G)$.

Now
$N = \{a\in G: \lambda_a = \id\} = \{a\in G: ax = x \text{ for all } x \in G\} = \{e\}$.
Therefore, $N = \{e\}$, and so $G \cong G/N$.  If $\pi: G \rightarrow G/N$
denotes this isomorphism, we have 
$\psi\circ \pi : G \rightarrow G/N \rightarrow \Sym(G)$.  Since $\psi$ and $\pi$
are both one-to-one in this case, we have an isomorphism between $G$ and the
subgroup $(\psi\circ \pi)(G)$ of $\Sym(G)$.  That is $G$ is isomorphic to a
subgroup of $\Sym(G)$.
\newpage

\item Let $\bS = \<S, \cdot\>$ and $\bT = \<T, \circ\>$ be two semilattices.
  \begin{enumerate}
  \item Say what it means for a function $\varphi: S \rightarrow T$ to be a
    \emph{semilattice homomorphism} $\varphi: \bS \rightarrow \bT$.

\medskip

A function $\varphi: S \rightarrow T$ is
a \emph{semilattice homomorphism} if  
$\varphi(x\cdot y) = \varphi(x) \circ \varphi(y)$
holds for all $x, y \in S$.

\bigskip

\item Let $S = \{a, b, c, d\}$ and $T = \{0, 1, 2\}$, and suppose 
  $\bS = \<S, \cdot\>$ and
  $\bT= \<T, \circ\>$ have the Cayley tables given below

\medskip
\begin{center}
\begin{tabular}{r|rrrr}
  $\cdot$ & $a$ &$b$&$c$&$d $\\
\hline
  $a$ & $a$ &$a$&$a$&$a$\\
  $b$ & $a$ &$b$&$a$&$b$\\
  $c$ & $a$ &$a$&$c$&$c$\\
  $d$ & $a$ &$b$&$c$&$d$
\end{tabular}
\hskip2cm
\begin{tabular}{r|rrr}
  $\circ$ & $0$ &$1$&$2$\\
\hline
  $0$ & $0$ &$0$&$0$\\
  $1$ & $0$ &$1$&$1$\\
  $2$ & $0$ &$1$&$2$
\end{tabular}
\end{center}

\medskip
The Hasse diagrams of $\bS$ and $\bT$ are as follows:
\begin{center}
  
\begin{tikzpicture}[scale=0.6]
  \node (0) at (0,0) [draw, inner sep=1pt] {};
  \node (1) at (1.5,2)[draw,circle,inner sep=1pt] {}; 
  \node (2) at (-1.5,2) [draw,circle,inner sep=1pt] {};
  \node (3) at (0,4) [draw,circle,inner sep=1pt] {};
  \node (a) at (4,0) [draw,circle,inner sep=1pt] {};
  \node (b) at (4,2) [draw,circle,inner sep=1pt] {};
  \node (c) at (4,4) [draw,circle,inner sep=1pt] {};
  \draw (a) to (b) to (c);
  \draw (0) to (1) to (3) to (2) to (0);

  \draw (0) node [below] {$a$};
  \draw (2) node [left] {$b$};
  \draw (1) node [right] {$c$};
  \draw (3) node [above] {$d$};
  \draw (a) node [right] {$0$};
  \draw (b) node [right] {$1$};
  \draw (c) node [right] {$2$};
\end{tikzpicture}
\end{center}

Determine which of the functions $\varphi_i$ defined below is a homomorphism.
In case $\varphi_i$ is not a homomorphism, give an example of 
a violation of the definition in Part (a).

\medskip
\begin{center}
\begin{tabular}{c|c}
  $x$ & $\varphi_1(x)$ \\
\hline
  $a$ & $0$\\\hline
  $b$ & $1$\\\hline
  $c$ & $0$\\\hline
  $d$ & $1$
\end{tabular}
\hskip3cm
\begin{tabular}{c|c}
  $x$ & $\varphi_2(x)$ \\
\hline
  $a$ & $0$\\\hline
  $b$ & $1$\\\hline
  $c$ & $1$\\\hline
  $d$ & $2$
\end{tabular}
%% \hskip2cm
%% \begin{tabular}{c|c}
%%   $x$ & $\varphi_3(x)$ \\
%% \hline
%%   $a$ & $1$\\\hline
%%   $b$ & $1$\\\hline
%%   $c$ & $2$\\\hline
%%   $d$ & $2$
%% \end{tabular}
\end{center}

\medskip

The function $\varphi_1$ is a homomorphism. For all $s\in S$, we have 
\[
\varphi_1(a\cdot s) = \varphi(a) = 0 = 0 \circ \varphi(s) = \varphi(a) \circ
\varphi(s).\]
Also, $\varphi_1(b\cdot c) = \varphi(a) = 0 = \varphi_1(b) \circ 0 = \varphi_1(b) \circ \varphi_1(c),$
and
\[\varphi_1(b\cdot d) = \varphi(b) = 1 = 1\circ 1 = \varphi_1(b) \circ
\varphi_1(d), \text{ and }\]
\[\varphi_1(c\cdot d) = \varphi(c) = 0 = 1\circ 1 = \varphi_1(b) \circ
\varphi_1(d).\]
These facts, and commutativity, imply that 
$\varphi(x \cdot y) = \varphi(x) \circ \varphi(y)$ for all $x, y \in S$.  

\medskip

The function $\varphi_2$ is not a homomorphism.  For example, 
\[\varphi(b\cdot c) = \varphi(a) = 0 \neq 1 = \varphi(b) \circ \varphi(c).\]

\end{enumerate}


  \end{enumerate}
\newpage
\begin{center}
  EXTRA CREDIT
\end{center}
Below I have drawn the subgroup lattice diagrams for the groups $\Z_2$,
$\Z_7$, $\Z_{12}$, $\Z_{16}$, $\Z_{30}$, $S_3$, and  $D_4/Z(D_4)$ but I've
forgotten which diagram go with which group.  I was able to label the first
diagram correctly.  If you think you can help me label the others, go for
it. But don't guess. 

\medskip

{\it $+1$ point for each correct answer, $-1/4$ point for each incorrect answer.} 
%\begin{multicols}{2}

\bigskip

\begin{center}
% Z_2
\begin{tikzpicture}[scale=1.25]
  \node (bot) at (0,0) [draw,circle,inner sep=1pt] {};
  \node (top) at (0,2) [draw,circle,inner sep=1pt] {};
  \draw (bot) to (top);
  \node (G) at (0,-1) {$G = \Z_2$};
  \node (line) at (.1,-1.2) {\underline{\phantom{XXXXXXX}}};
\end{tikzpicture}
\hskip3cm
% Z_7
\begin{tikzpicture}[scale=1.25]
  \node (bot) at (0,0) [draw,circle,inner sep=1pt] {};
  \node (top) at (0,2) [draw,circle,inner sep=1pt] {};
  \draw (bot) to (top);
  \node (G) at (0,-1) {$\Z_7$};
  \node (line) at (0,-1.2) {\underline{\phantom{XXXXXXX}}};
\end{tikzpicture}
% Z_16
\hskip3cm
\begin{tikzpicture}[scale=1.25]
  \node (bot) at (0,0) [draw,circle,inner sep=1pt] {};
  \node (1) at (0,1) [draw,circle,inner sep=1pt] {};
  \node (top) at (0,2) [draw,circle,inner sep=1pt] {};
  \draw (bot) to (1) to (top);
  \node (G) at (0,-1) {$\Z_{16}$};
  \node (line) at (0,-1.2) {\underline{\phantom{XXXXXXX}}};
\end{tikzpicture}
\end{center}
\vskip1cm
\begin{center}
\begin{tikzpicture}[scale=1.25]
  \node (bot) at (0,0) [draw,circle,inner sep=1pt] {};
  \node (1) at (1,1) [draw,circle,inner sep=1pt] {};
  \node (2) at (-1,1) [draw,circle,inner sep=1pt] {};
  \node (3) at (0,1) [draw,circle,inner sep=1pt] {};
  \node (top) at (0,2) [draw,circle,inner sep=1pt] {};
  \draw (bot) to (1) to (top) to (2) to (bot) to (3) to (top);
  \node (G) at (0,-1) {$D_4/Z(D_4)$};
  \node (line) at (0,-1.2) {\underline{\phantom{XXXXXXXX}}};
\end{tikzpicture}
\hskip3cm
\begin{tikzpicture}[scale=1.25]
  \node (bot) at (0,0) [draw,circle,inner sep=1pt] {};
  \node (1) at (1.5,1) [draw,circle,inner sep=1pt] {};
  \node (2) at (-1.5,1) [draw,circle,inner sep=1pt] {};
  \node (3) at (.7,1) [draw,circle,inner sep=1pt] {};
  \node (4) at (-.7,1) [draw,circle,inner sep=1pt] {};
  \node (top) at (0,2) [draw,circle,inner sep=1pt] {};
  \draw (bot) to (1) to (top) to (2) to (bot) to (3) to (top) to (4) to (bot);
  \node (G) at (0,-1) {$S_3$};
  \node (line) at (0,-1.2) {\underline{\phantom{XXXXXXX}}};
%  \node (G) at (0,-1.5) {$G =$};
\end{tikzpicture}
\end{center}
\vskip1cm
\begin{center}
\begin{tikzpicture}[scale=0.7]
  \node (1) at (0,0) [draw,circle,inner sep=1pt] {};
  \node (6) at (2,2)[draw,circle,inner sep=1pt] {}; 
  \node (4) at (-2,2) [draw,circle,inner sep=1pt] {};
  \node (2) at (0,4) [draw,circle,inner sep=1pt] {};
  \node (3) at (4,4) [draw,circle,inner sep=1pt] {};
  \node (G) at (2,6) [draw,circle,inner sep=1pt] {};
  \draw (1) to (6) to (2) to (4) to (1);
  \draw (6) to (3) to (G) to (2) to (4);
  \node (G) at (1,-1) {$\Z_{12}$};
  \node (line) at (1,-1.2) {\underline{\phantom{XXXXXXX}}};
%  \node (G) at (0,-1.5) {$G =$};
\end{tikzpicture}
\hskip3cm
\begin{tikzpicture}[scale=0.55]
  \node (e) at (0,0)  [draw,circle,inner sep=1pt] {};
  \node (G) at (0,8) [draw,circle,inner sep=1pt] {};
  \node (2) at (-3,6) [draw,circle,inner sep=1pt] {};
  \node (3) at (0,5)  [draw,circle,inner sep=1pt] {};
  \node (5) at (3,6) [draw,circle,inner sep=1pt] {}; 
  \node (6) at (-3,2.5) [draw,circle,inner sep=1pt] {};
  \node (10) at (0,3)  [draw,circle,inner sep=1pt] {};
  \node (15) at (3,2.5)  [draw,circle,inner sep=1pt] {};
  \node (Group) at (1,-1) {$\Z_{30}$};
  \node (line) at (1,-1.4) {\underline{\phantom{XXXXXXX}}};
  \draw (e) to (15) to (3) to (6) to (e);
  \draw (e) to (10) to (5) to (G) to (2) to (10);
  \draw (6) to (2) (3) to (G) (15) to (5);
\end{tikzpicture}
\end{center}



\end{document}
